chore: Split automata theory translations into multiple files

Cslib/Computability/Automata/DFA.lean
@@ -17,7 +17,7 @@ a finite string.
 * [J. E. Hopcroft, R. Motwani, J. D. Ullman, *Introduction to Automata Theory, Languages, and Computation*][Hopcroft2006]
 -/
 
-/-- A Deterministic Finite-State Automaton (DFA) consists of a labelled transition function
+/-- A Deterministic Finite Automaton (DFA) consists of a labelled transition function
 `tr` over finite sets of states and labels (called symbols), a starting state `start` and a finite
 set of accepting states `accept`. -/
 structure DFA (State : Type _) (Symbol : Type _) extends DA State Symbol where
@@ -25,3 +25,35 @@ structure DFA (State : Type _) (Symbol : Type _) extends DA State Symbol where
   finite_state : Finite State
   /-- The type of symbols (also called 'alphabet') is finite. -/
   finite_symbol : Finite Symbol
+
+
+namespace DFA
+
+/-- Extended transition function.
+
+Implementation note: compared to [Hopcroft2006], the definition consumes the input list of symbols
+from the left (instead of the right), in order to match the way lists are constructed.
+-/
+@[grind]
+def mtr (dfa : DFA State Symbol) (s : State) (xs : List Symbol) := xs.foldl dfa.tr s
+
+@[grind]
+theorem mtr_nil_eq {dfa : DFA State Symbol} : dfa.mtr s [] = s := by rfl
+
+/-- A DFA accepts a string if there is a multi-step accepting derivative with that trace from
+the start state. -/
+@[grind]
+def Accepts (dfa : DFA State Symbol) (xs : List Symbol) :=
+  (dfa.mtr dfa.start xs) ∈ dfa.accept
+
+/-- The language of a DFA is the set of strings that it accepts. -/
+@[grind]
+def language (dfa : DFA State Symbol) : Set (List Symbol) :=
+  { xs | dfa.Accepts xs }
+
+/-- A string is accepted by a DFA iff it is in the language of the DFA. -/
+@[grind]
+theorem accepts_mem_language (dfa : DFA State Symbol) (xs : List Symbol) :
+  dfa.Accepts xs ↔ xs ∈ dfa.language := by rfl
+
+end DFA
