Cslib/Computability/Automata/NA.lean
@@ -19,23 +19,3 @@ structure NA (State : Type _) (Symbol : Type _) extends LTS State Symbol where
   start : Set State
   /-- The set of accepting states of the automaton. -/
   accept : Set State
-
-namespace NA
-
-/-- An NA accepts a string if there is a multi-step accepting derivative with that trace from
-the start state. -/
-@[grind]
-def Accepts (na : NA State Symbol) (xs : List Symbol) :=
-  ∃ s ∈ na.start, ∃ s' ∈ na.accept, na.MTr s xs s'
-
-/-- The language of a DA is the set of strings that it accepts. -/
-@[grind]
-def language (na : NA State Symbol) : Set (List Symbol) :=
-  { xs | na.Accepts xs }
-
-/-- A string is accepted by an NA iff it is in the language of the NA. -/
-@[grind]
-theorem accepts_mem_language (na : NA State Symbol) (xs : List Symbol) :
-  na.Accepts xs ↔ xs ∈ na.language := by rfl
-
-end NA
