Cslib/Computability/Automata/NFA.lean
@@ -6,10 +6,30 @@ Authors: Fabrizio Montesi
 
 import Cslib.Computability.Automata.NA
 
-/-- A Nondeterministic Finite-State Automaton (NFA) is a nondeterministic automaton (NA)
+/-- A Nondeterministic Finite Automaton (NFA) is a nondeterministic automaton (NA)
 over finite sets of states and symbols. -/
 structure NFA (State : Type _) (Symbol : Type _) extends NA State Symbol where
   /-- The automaton is finite-state. -/
   finite_state : Finite State
   /-- The type of symbols (also called 'alphabet') is finite. -/
   finite_symbol : Finite Symbol
+
+namespace NFA
+
+/-- An NFA accepts a string if there is a multi-step accepting derivative with that trace from
+the start state. -/
+@[grind]
+def Accepts (nfa : NFA State Symbol) (xs : List Symbol) :=
+  ∃ s ∈ nfa.start, ∃ s' ∈ nfa.accept, nfa.MTr s xs s'
+
+/-- The language of an NFA is the set of strings that it accepts. -/
+@[grind]
+def language (nfa : NFA State Symbol) : Set (List Symbol) :=
+  { xs | nfa.Accepts xs }
+
+/-- A string is accepted by an NFA iff it is in the language of the NFA. -/
+@[grind]
+theorem accepts_mem_language (nfa : NFA State Symbol) (xs : List Symbol) :
+  nfa.Accepts xs ↔ xs ∈ nfa.language := by rfl
+
+end NFA
