Cslib/Computability/Automata/DFAToNFA.lean
@@ -1,0 +1,75 @@
+/-
+Copyright (c) 2025 Fabrizio Montesi. All rights reserved.
+Released under Apache 2.0 license as described in the file LICENSE.
+Authors: Fabrizio Montesi
+-/
+
+import Cslib.Computability.Automata.DFA
+import Cslib.Computability.Automata.NFA
+
+/-! # Translation of DFA into NFA -/
+
+namespace DFA
+section NFA
+
+/-- `DFA` is a special case of `NFA`. -/
+@[grind =]
+def toNFA (dfa : DFA State Symbol) : NFA State Symbol := {
+  start := {dfa.start}
+  accept := dfa.accept
+  Tr := fun s1 μ s2 => dfa.tr s1 μ = s2
+  finite_state := dfa.finite_state
+  finite_symbol := dfa.finite_symbol
+}
+
+@[grind =]
+lemma toNFA_start {dfa : DFA State Symbol} : dfa.toNFA.start = {dfa.start} := rfl
+
+instance : Coe (DFA State Symbol) (NFA State Symbol) where
+  coe := toNFA
+
+/-- `DA.toNA` correctly characterises transitions. -/
+@[grind]
+theorem toNA_tr {dfa : DFA State Symbol} :
+  dfa.toNFA.Tr s1 μ s2 ↔ dfa.tr s1 μ = s2 := by
+  rfl
+
+/-- The transition system of a DA is deterministic. -/
+@[grind]
+theorem toNFA_deterministic (dfa : DFA State Symbol) : dfa.toNFA.Deterministic := by
+  grind
+
+/-- The transition system of a DA is image-finite. -/
+@[grind]
+theorem toNFA_imageFinite (dfa : DFA State Symbol) : dfa.toNFA.ImageFinite :=
+  dfa.toNFA.deterministic_imageFinite dfa.toNFA_deterministic
+
+/-- Characterisation of multistep transitions. -/
+@[grind]
+theorem toNFA_mtr {dfa : DFA State Symbol} :
+  dfa.toNFA.MTr s1 xs s2 ↔ dfa.mtr s1 xs = s2 := by
+  constructor <;> intro h
+  case mp =>
+    induction h <;> grind
+  case mpr =>
+    induction xs generalizing s1
+    case nil => grind
+    case cons x xs ih =>
+      apply LTS.MTr.stepL (s2 := dfa.tr s1 x) <;> grind
+
+/-- The `NFA` constructed from a `DFA` has the same language. -/
+@[grind]
+theorem toNFA_language_eq {dfa : DFA State Symbol} :
+  dfa.toNFA.language = dfa.language := by
+  ext xs
+  rw [← DFA.accepts_mem_language, ← NFA.accepts_mem_language]
+  simp only [NFA.Accepts, DFA.Accepts]
+  apply Iff.intro <;> intro h
+  case mp =>
+    grind
+  case mpr =>
+    exists dfa.start
+    grind
+
+end NFA
+end DFA
