Cslib/Computability/Automata/EpsilonNFAToNFA.lean
@@ -1,0 +1,89 @@
+/-
+Copyright (c) 2025 Fabrizio Montesi. All rights reserved.
+Released under Apache 2.0 license as described in the file LICENSE.
+Authors: Fabrizio Montesi
+-/
+
+import Cslib.Computability.Automata.EpsilonNFA
+import Cslib.Computability.Automata.NFA
+
+/-! # Translation of εNFA into NFA -/
+
+/-- Converts an `LTS` with Option labels into an `LTS` on the carried label type, by removing all
+ε-transitions. -/
+@[grind]
+private def LTS.noε (lts : LTS State (Option Label)) :
+  LTS State Label := {
+  Tr := fun s μ s' => lts.Tr s (some μ) s'
+}
+
+@[grind]
+private lemma LTS.noε_saturate_tr
+  {lts : LTS State (Option Label)} {h : μ = some μ'} :
+  lts.saturate.Tr s μ s' ↔ lts.saturate.noε.Tr s μ' s' := by
+  simp only [LTS.noε]
+  grind
+
+namespace εNFA
+
+section NFA
+
+/-- Any εNFA can be converted into an NFA that does not use ε-transitions. -/
+@[grind]
+def toNFA (enfa : εNFA State Symbol) : NFA State Symbol := {
+  start := enfa.εClosure enfa.start
+  accept := enfa.accept
+  Tr := enfa.saturate.noε.Tr
+  finite_state := enfa.finite_state
+  finite_symbol := enfa.finite_symbol
+}
+
+@[grind]
+lemma LTS.noε_saturate_mTr
+  {lts : LTS State (Option Label)} :
+  lts.saturate.MTr s (μs.map (some ·)) = lts.saturate.noε.MTr s μs := by
+  ext s'
+  induction μs generalizing s
+  case nil => grind
+  case cons μ μs ih =>
+    apply Iff.intro <;> intro h
+    case mp =>
+      simp only [LTS.noε]
+      cases h
+      rename_i sb htr hmtr
+      apply LTS.MTr.stepL (s1 := s) (s2 := sb) (s3 := s') <;> grind
+    case mpr =>
+      simp only [LTS.noε] at h
+      grind
+
+
+/-- Correctness of `toNAWithoutEpsilon`. -/
+@[grind]
+theorem toNAWithoutEpsilon_language_eq {enfa : εNFA State Symbol} :
+  enfa.toNFA.language = enfa.language := by
+  ext xs
+  apply Iff.intro
+  case mp =>
+    rw [← εNFA.accepts_mem_language, ← NFA.accepts_mem_language]
+    simp only [NFA.Accepts, toNFA, Accepts, forall_exists_index, and_imp]
+    intro s hs s' hs' hmtr
+    exists s
+    apply And.intro hs
+    exists s'
+    apply And.intro hs'
+    rw [LTS.noε_saturate_mTr]
+    assumption
+  case mpr =>
+    rw [← εNFA.accepts_mem_language, ← NFA.accepts_mem_language]
+    simp only [NFA.Accepts, toNFA, Accepts, forall_exists_index, and_imp]
+    intro s hs s' hs' hmtr
+    exists s
+    apply And.intro hs
+    exists s'
+    apply And.intro hs'
+    rw [← LTS.noε_saturate_mTr]
+    assumption
+
+end NFA
+
+end εNFA
